platform/cito/examples/Factorial.v
@@ -8,45 +8,74 @@ Export Wrp.
 Require Import Notations4.
 Module Import Notations4Make := Make ExampleADT.
 
-Definition fact_partial_w (a b : W) : W := $0.
+Open Scope nat.
 
-(*
-    ([  ]
-    While (0 < "n") {
-      "ret" <- "ret" * "n" ;;
-      "n" <- "n" - 1                          
-    })%SP.
+Require Import Arith.
 
-Require Import AutoSep.
+Definition fact_w (w : W) := natToW (fact (wordToNat w)).
 
-Require Import Notations4.
+Fixpoint fact_partial' start n :=
+  match n with
+    | 0 => 1
+    | S n' => start * fact_partial' (1 + start) n'
+  end.
 
-Definition s :=
-([
-      PRE[V] Emp
-      POST[R] Emp ]
-    While ("x" <> 0) {
-      "tmp2" <- "x";;
-      "tmp1" <- "x" + 4;;
-      "x" <-* "tmp1";;
-      "tmp1" *<- "acc";;
-      "acc" <- "tmp2"
-    })%SP.
+(* (a+1) * (a+2) * ... * b  (1 when a>=b) *)
+Definition fact_partial (a b : nat) := fact_partial' (1 + a) (b - a).
 
-*)
+Definition fact_partial_w (a b : W) : W := natToW (fact_partial (wordToNat a) (wordToNat b)).
+
+Set Printing Coercions.
+
+Lemma fact_partial_0 : forall n, fact_partial 0 n = fact n.
+  unfold fact_partial.
+  induction n; simpl; intuition.
+  rewrite plus_0_r in *.
+  Require Import NPeano.
+  Import NPeano.Nat.
+  rewrite sub_0_r in *.
+  Lemma fact_partial'_inv : forall n start, fact_partial' start n * (n + start) = start * fact_partial' (1 + start) n.
+    Opaque mult.
+    induction n; simpl; intuition.
+    repeat rewrite <- IHn.
+    rewrite mult_assoc.
+    repeat rewrite <- IHn.
+    ring.
+    Transparent mult.
+  Qed.
+  specialize (fact_partial'_inv n 1); intro; simpl in *.
+  rewrite plus_0_r in *.
+  rewrite <- H.
+  rewrite IHn.
+  ring.
+Qed.
+
+Lemma fact_partial_w_0 : forall w, fact_partial_w $0 w = fact_w w.
+  intros.
+  unfold fact_partial_w, fact_w.
+  f_equal.
+  change (wordToNat $0) with 0.
+  eapply fact_partial_0.
+Qed.
+
+Lemma fact_partial_w_same : forall w, fact_partial_w w w = 1.
+  admit.
+Qed.
 
 Import ProgramLogicMake.
 
-Definition f := (
-  cfunction "fact"("n0") (
-    "n" <- "n0" ;;
+Definition body := (
     "ret" <- 1 ;;
-    [ fun v => sel (fst v) "ret" = fact_partial_w (sel (fst v) "n") (sel (fst v) "n0") ]
+    [ fun v0 v => sel (fst v) "ret" = fact_partial_w (sel (fst v) "n") (sel (fst v0) "n") /\ snd v = snd v0 ]
     While (0 < "n") {
       "ret" <- "ret" * "n" ;;
       "n" <- "n" - 1                          
     }
-  )%stmtex
+  )%stmtex.
+
+Definition f := (
+  cfunction "fact"("n")
+    body            
   end
 )%Citofuncs.
 
@@ -70,14 +99,6 @@ Notation extra_stack := 100.
 Definition topS := SPEC reserving (4 + extra_stack)
   PREonly[_] mallocHeap 0.
 
-Fixpoint fact n :=
-  match n with
-    | 0 => 1
-    | S n' => (n * fact n')%nat
-  end.
-
-Definition fact_w (w : W) := natToW (fact (wordToNat w)).
-
 Notation input := 5.
 
 Definition top := bimport [[ ("fact"!"fact", fspec), "sys"!"printInt" @ [printIntS],
@@ -97,15 +118,79 @@ Definition top := bimport [[ ("fact"!"fact", fspec), "sys"!"printInt" @ [printIn
 
 Import LinkSpecMake.
 
-Lemma body_safe : forall stn fs v, stn_good_to_use (gm :: nil) (empty _) stn -> fs_good_to_use (gm :: nil) (empty _) fs stn -> Safe (from_bedrock_label_map (Labels stn), fs stn) (Body f) v.
+Lemma body_runsto : forall stn fs v v', stn_good_to_use (gm :: nil) (empty _) stn -> fs_good_to_use (gm :: nil) (empty _) fs stn -> RunsTo (from_bedrock_label_map (Labels stn), fs stn) (Body f) v v' -> sel (fst v') (RetVar f) = fact_w (sel (fst v) "n") /\ snd v' = snd v.
+  intros.
+  unfold f in *; simpl in *.
+  eapply sound_runsto' with (p := fun v0 v => v0 = v) in H1.
+  2 : instantiate (1 := body); simpl; eauto.
+  simpl in *.
+  unfold and_lift, interp, abs in *.
+  openhyp.
+  split.
+  2 : eauto.
+  rewrite H1.
+  replace (sel (fst v') "n") with (natToW 0).
+  eapply fact_partial_w_0.
+  unfold is_false, abs in *; simpl in *.
+  unfold wltb in *.
+  destruct wlt_dec; try discriminate.
+  Close Scope nat.
+  Lemma wle_0_eq : forall w : W, w <= $0 -> w = $0.
+    intros.
+    unfold wlt in *.
+    destruct (N.eq_0_gt_0_cases (wordToN w)).
+    change (0)%N with (wordToN (natToW 0)) in H0.
+    eapply wordToN_inj in H0.
+    eauto.
+    change (wordToN ($ 0)) with 0%N in H.
+    intuition.
+  Qed.
+  symmetry.
+  eapply wle_0_eq; eauto.
+  simpl in *.
+  unfold imply_close, and_lift, interp, abs.
+  descend.
+  openhyp.
+  subst.
+  simpl.
+  split.
+  rewrite sel_upd_ne by eauto.
+  rewrite H3.
+  symmetry; eapply fact_partial_w_same.
+  eauto.
+  openhyp; simpl in *.
+  destruct v0; destruct v'0; simpl in *.
+  Lemma sel_upd_eq' : forall vs nm v nm', nm = nm' -> (upd vs nm v) nm' = v.
+    intros; eapply sel_upd_eq; eauto.
+  Qed.
+  Lemma sel_upd_ne' : forall vs nm v nm', nm <> nm' -> (upd vs nm v) nm' = sel vs nm'.
+    intros; eapply sel_upd_ne; eauto.
+  Qed.
+  Ltac sel_upd_simpl :=
+    repeat 
+      match goal with
+        | H : _ |- _ => rewrite sel_upd_eq in H by reflexivity
+        | H : _ |- _ => rewrite sel_upd_ne in H by discriminate
+        | |- _ => rewrite sel_upd_eq by reflexivity
+        | |- _ => rewrite sel_upd_ne by discriminate
+        | H : _ |- _ => rewrite sel_upd_eq' in H by reflexivity
+        | H : _ |- _ => rewrite sel_upd_ne' in H by discriminate
+        | |- _ => rewrite sel_upd_eq' by reflexivity
+        | |- _ => rewrite sel_upd_ne' by discriminate
+      end.
+  sel_upd_simpl.
+  subst.
+  split.
+  rewrite H4.
+  rewrite H3.
   admit.
+  eauto.
+  eauto.
+  unfold interp.
+  eauto.
 Qed.
 
-Lemma body_runsto : forall stn fs v v', stn_good_to_use (gm :: nil) (empty _) stn -> fs_good_to_use (gm :: nil) (empty _) fs stn -> RunsTo (from_bedrock_label_map (Labels stn), fs stn) (Body f) v v' -> sel (fst v') (RetVar f) = fact_w (sel (fst v) "n0") /\ snd v' = snd v.
-  intros.
-  eapply sound in H1.
-  unfold f in *; simpl in *.
-
+Lemma body_safe : forall stn fs v, stn_good_to_use (gm :: nil) (empty _) stn -> fs_good_to_use (gm :: nil) (empty _) fs stn -> Safe (from_bedrock_label_map (Labels stn), fs stn) (Body f) v.
   admit.
 Qed.
 
@@ -123,7 +208,8 @@ Theorem top_ok : moduleOk top.
   sep_auto.
 
   post.
-  call_cito 100 ("n0" :: nil).
+  Open Scope nat.
+  call_cito 100 ("n" :: nil).
   hiding ltac:(evaluate auto_ext).
   unfold name_marker.
   hiding ltac:(step auto_ext).
@@ -132,7 +218,7 @@ Theorem top_ok : moduleOk top.
   descend.
   eapply CompileExprs.change_hyp.
   Focus 2.
-  apply (@is_state_in''' (upd (upd x2 "extra_stack" 100) "n0" input)).
+  apply (@is_state_in''' (upd (upd x2 "extra_stack" 100) "n" input)).
   autorewrite with sepFormula.
   hiding ltac:(step auto_ext).
   apply body_safe; eauto.
@@ -146,7 +232,7 @@ Theorem top_ok : moduleOk top.
   end.
   apply body_runsto in H9; simpl in H9; intuition subst.
   eapply replace_imp.
-  change 100 with (wordToNat (sel (upd (upd x2 "extra_stack" 100) "n0" 5) "extra_stack")).
+  change 100 with (wordToNat (sel (upd (upd x2 "extra_stack" 100) "n" 5) "extra_stack")).
   apply is_state_out''''.
   NoDup.
   NoDup.
